PalamedesTest/Corpus/Range/BetweenLoAndHi.lean
@@ -2,5 +2,5 @@ import Palamedes.Synthesizer
 
 open Palamedes Palamedes.Gen Palamedes.Gen.CorrectGen
 
-def genBetweenLoAndHi (lo hi : Nat) : Gen Nat := by
-  generator_search (fun n => lo ≤ n ∧ n ≤ hi) allow_partial
+def genBetweenLoAndHi (lo hi : Nat) [_root_.Gen G] : G (Option Nat) := by
+  generator_search (fun n => lo ≤ n ∧ n ≤ hi)
