Palamedes/Synthesizer.lean
@@ -1,1 +1,2 @@
 import Palamedes.Synthesizer.FrontEnd
+import Palamedes.Synthesizer.CorrectDef
